src/Init/Data/List/Attach.lean
@@ -568,22 +568,22 @@ If not, usually the right approach is `simp [List.unattach, -List.map_subtype]` 
 -/
 def unattach {α : Type _} {p : α → Prop} (l : List { x // p x }) := l.map (·.val)
 
-@[simp] theorem unattach_nil {α : Type _} {p : α → Prop} : ([] : List { x // p x }).unattach = [] := rfl
-@[simp] theorem unattach_cons {α : Type _} {p : α → Prop} {a : { x // p x }} {l : List { x // p x }} :
+@[simp] theorem unattach_nil {p : α → Prop} : ([] : List { x // p x }).unattach = [] := rfl
+@[simp] theorem unattach_cons {p : α → Prop} {a : { x // p x }} {l : List { x // p x }} :
   (a :: l).unattach = a.val :: l.unattach := rfl
 
-@[simp] theorem length_unattach {α : Type _} {p : α → Prop} {l : List { x // p x }} :
+@[simp] theorem length_unattach {p : α → Prop} {l : List { x // p x }} :
     l.unattach.length = l.length := by
   unfold unattach
   simp
 
-@[simp] theorem unattach_attach {α : Type _} (l : List α) : l.attach.unattach = l := by
+@[simp] theorem unattach_attach {l : List α} : l.attach.unattach = l := by
   unfold unattach
   induction l with
   | nil => simp
   | cons a l ih => simp [ih, Function.comp_def]
 
-@[simp] theorem unattach_attachWith {α : Type _} {p : α → Prop} {l : List α}
+@[simp] theorem unattach_attachWith {p : α → Prop} {l : List α}
     {H : ∀ a ∈ l, p a} :
     (l.attachWith p H).unattach = l := by
   unfold unattach
